Add Find and Map.

src/dafny/utils/MiscTypes.dfy
@@ -61,10 +61,10 @@ module MiscTypes {
   function {:tailrecursion true} Filter<U>(u: seq<U>, f: U -> bool): (r: seq<U>)
     ensures |r| <= |u|
     ensures forall x:: x in r ==> x in u
-    ensures forall k:: 0 <= k < |r| ==> f(r[k]) 
+    ensures forall k:: 0 <= k < |r| ==> f(r[k])
     ensures forall x:: x in r ==> f(x)
   {
-    if |u| == 0 then [] 
+    if |u| == 0 then []
     else if f(u[0]) then [u[0]] + Filter(u[1..], f)
     else Filter(u[1..], f)
   }
@@ -73,9 +73,41 @@ module MiscTypes {
     ensures !Exists(xs, f) ==> forall k:: k in xs ==> !f(k)
     ensures !Exists(xs, f) ==> forall k:: 0 <= k < |xs| ==> !f(xs[k])
   {
-    if |xs| == 0 then false 
+    if |xs| == 0 then false
     else if f(xs[0]) then true
     else Exists(xs[1..], f)
+  }
+
+  /**   Map each value of a seq according to a function. */
+  function Map<T, U>(t: seq<T>, f: T -> U): seq<U>
+    ensures |t| == |Map(t, f)|
+    ensures forall i:: 0 <= i < |t| ==> Map(t, f)[i] == f(t[i])
+  {
+    seq(|t|, i requires 0 <= i < |t| => f(t[i]))
+  }
+
+  /** Find the index of an element in a list.  */
+  function Find<T(==)>(x: seq<T>, t: T): Option<nat>
+    ensures Find(x, t).Some? <==> t in x
+    ensures Find(x, t).Some? ==> Find(x, t).Extract() < |x|
+    ensures Find(x, t).Some? ==> x[Find(x, t).Extract()] == t
+    ensures Find(x, t).None? <==> t !in x
+  {
+    FindRec(x, t)
+  }
+
+  function {:tailrecursion true} FindRec<T(==)>(x: seq<T>, t: T, i: nat := 0, ghost c: seq<T> := x): Option<nat>
+    requires |c| == i + |x|
+    requires c[i..] == x
+    ensures FindRec(x, t, i, c).Some? ==> t in c
+    ensures FindRec(x, t, i, c).Some? ==> FindRec(x, t, i, c).Extract() < |c|
+    ensures FindRec(x, t, i, c).Some? ==> c[FindRec(x, t, i, c).Extract()] == t
+    ensures FindRec(x, t, i, c).None? <==> t !in x
+    decreases |x|
+  {
+    if |x| == 0 then None
+    else if x[0] == t then Some(i)
+    else FindRec(x[1..], t, i + 1, c)
   }
 
 }
